Tests/DTLC/TrmSpec.lean
@@ -29,49 +29,49 @@ end eraseType
 section eval
 
 example :
-    ((Trm.vFalse : Trm).eval).yields
+    ((Trm.vFalse : Trm).eval).shouldYields
       ((.primitive "false") : Val) := by
   constructor
   · exact ⟨1, rfl⟩
   · rfl
 
 example :
-    ((Trm.idFnOnFalse : Trm).eval).yields
+    ((Trm.idFnOnFalse : Trm).eval).shouldYields
       ((.primitive "false") : Val) := by
   constructor
   · exact ⟨2, by simp [AST.Trm.eval, idFnOnFalse, idFn, vFalse]⟩
   · rfl
 
 example :
-    ((Trm.get1stOnTuple : Trm).eval).yields
+    ((Trm.get1stOnTuple : Trm).eval).shouldYields
       ((.primitive "false") : Val) := by
   constructor
   · exact ⟨3, by simp [AST.Trm.eval, get1stOnTuple, get1st, vFalse, vTrue]⟩
   · rfl
 
 example :
-    ((Trm.get2ndOnTuple : Trm).eval).yields
+    ((Trm.get2ndOnTuple : Trm).eval).shouldYields
       ((.primitive "true") : Val) := by
   constructor
   · exact ⟨3, by simp [AST.Trm.eval, get2ndOnTuple, get2nd, vFalse, vTrue]⟩
   · rfl
 
 example :
-    ((Trm.apply1stOn2ndFnOnTuple : Trm).eval).yields
+    ((Trm.apply1stOn2ndFnOnTuple : Trm).eval).shouldYields
       ((.primitive "false") : Val) := by
   constructor
   · exact ⟨4, by simp [AST.Trm.eval, apply1stOn2ndFnOnTuple, apply1stOn2ndFn, idFn, vFalse]⟩
   · rfl
 
 example :
-    ((Trm.applyidFnOnItself : Trm).eval).yields
+    ((Trm.applyidFnOnItself : Trm).eval).shouldYields
       (Val.idFn : Val) := by
   constructor
   · exact ⟨2, by simp [AST.Trm.eval, applyidFnOnItself, idFn, Val.idFn]⟩
   · rfl
 
 example :
-    ((Trm.idFnOnFalse2 : Trm).eval).yields
+    ((Trm.idFnOnFalse2 : Trm).eval).shouldYields
       ((.primitive "false") : Val) := by
   constructor
   · exact ⟨3, by simp [AST.Trm.eval, idFnOnFalse2, applyidFnOnItself, idFn, vFalse]⟩
@@ -87,7 +87,7 @@ example: ((Trm.Malformed.apply1 : Trm).eval 3) = .error := by
   simp [AST.Trm.eval, Malformed.apply1, idFn, vFalse, vTrue]
 
 example :
-    ((Trm.primitiveTrueFnOnFalse : Trm).eval).yields
+    ((Trm.primitiveTrueFnOnFalse : Trm).eval).shouldYields
       ((.primitive "true") : Val) := by
   constructor
   · exact ⟨2, rfl⟩
@@ -98,76 +98,76 @@ end eval
 section compile
 
 example :
-    vFalse.compile.yields vFalse := by
+    vFalse.compile.shouldYields vFalse := by
   sorry
 
 example :
-    vTrue.compile.yields vTrue := by
+    vTrue.compile.shouldYields vTrue := by
   sorry
 
 example :
-    idFn.compile.yields idFn := by
+    idFn.compile.shouldYields idFn := by
   sorry
 
 example :
-    idFnOnFalse.compile.yields idFnOnFalse := by
+    idFnOnFalse.compile.shouldYields idFnOnFalse := by
   sorry
 
 example :
-    get1st.compile.yields get1st := by
+    get1st.compile.shouldYields get1st := by
   sorry
 
 example :
-    get2nd.compile.yields get2nd := by
+    get2nd.compile.shouldYields get2nd := by
   sorry
 
 example :
-    get1stOnTuple.compile.yields get1stOnTuple := by
+    get1stOnTuple.compile.shouldYields get1stOnTuple := by
   sorry
 
 example :
-    get2ndOnTuple.compile.yields get2ndOnTuple := by
+    get2ndOnTuple.compile.shouldYields get2ndOnTuple := by
   sorry
 
 example :
-    apply1stOn2ndFn.compile.yields apply1stOn2ndFn := by
+    apply1stOn2ndFn.compile.shouldYields apply1stOn2ndFn := by
   sorry
 
 example :
-    apply1stOn2ndFnOnTuple.compile.yields
+    apply1stOn2ndFnOnTuple.compile.shouldYields
       apply1stOn2ndFnOnTuple := by
   sorry
 
 example :
-    applyidFnOnItself.compile.yields applyidFnOnItself := by
+    applyidFnOnItself.compile.shouldYields applyidFnOnItself := by
   sorry
 
 example :
-    idFnOnFalse2.compile.yields idFnOnFalse2 := by
+    idFnOnFalse2.compile.shouldYields idFnOnFalse2 := by
   sorry
 
 
 example :
-    primitiveTrueFn.compile.yields primitiveTrueFn := by
+    primitiveTrueFn.compile.shouldYields primitiveTrueFn := by
   sorry
 
 example :
-    primitiveTrueFnOnFalse.compile.yields
+    primitiveTrueFnOnFalse.compile.shouldYields
       primitiveTrueFnOnFalse := by
   sorry
 
 example :
-    TypeHinted.hintedFalse.compile.yields
+    TypeHinted.hintedFalse.compile.shouldYields
       TypeHinted.hintedFalse.typeHint.eraseRecursively := by
   sorry
 
 example :
-    TypeHinted.hintedIdFn.compile.yields
+    TypeHinted.hintedIdFn.compile.shouldYields
       TypeHinted.hintedIdFn.typeHint.eraseRecursively := by
   sorry
 
 example :
-    TypeHinted.hintedIdFnOnFalse.compile.yields
+    TypeHinted.hintedIdFnOnFalse.compile.shouldYields
       TypeHinted.hintedIdFnOnFalse.typeHint.eraseRecursively := by
   sorry
 
